QED

code/experimental/SPARKLE/dist/Hacl_Impl_Sparkle.c
@@ -24,8 +24,6 @@
 
 #include "Hacl_Impl_Sparkle.h"
 
-uint32_t Hacl_Impl_Sparkle_size_word = (uint32_t)4U;
-
 uint32_t Hacl_Impl_Sparkle_vsize_rcon = (uint32_t)8U;
 
 const
@@ -36,55 +34,153 @@ Hacl_Impl_Sparkle_rcon[8U] =
     (uint32_t)0xBB1185EBU, (uint32_t)0x4F7C7B57U, (uint32_t)0xCFBFA1C8U, (uint32_t)0xC2B3293DU
   };
 
-void
-Hacl_Impl_Sparkle_xor_step(uint32_t l, uint32_t *b, uint32_t *tx, uint32_t *ty, uint32_t i)
-{
-  uint32_t xi = b[(uint32_t)2U * i];
-  uint32_t yi = b[(uint32_t)2U * i + (uint32_t)1U];
-  uint32_t tx_0 = tx[0U];
-  uint32_t ty_0 = ty[0U];
-  tx[0U] = xi ^ tx_0;
-  ty[0U] = yi ^ ty_0;
-}
-
 Spec_SPARKLE2_branch1 Hacl_Impl_Sparkle_xor(uint32_t l, uint32_t *b)
 {
   uint32_t tx = (uint32_t)0U;
   uint32_t ty = (uint32_t)0U;
-  for (uint32_t i = (uint32_t)0U; i < l >> (uint32_t)1U; i++)
+  for (uint32_t i = (uint32_t)0U; i < l; i++)
   {
-    Hacl_Impl_Sparkle_xor_step(l, b, &tx, &ty, i);
+    uint32_t xi = b[(uint32_t)2U * i];
+    uint32_t yi = b[(uint32_t)2U * i + (uint32_t)1U];
+    uint32_t tx_0 = tx;
+    uint32_t ty_0 = ty;
+    tx = xi ^ tx_0;
+    ty = yi ^ ty_0;
   }
   uint32_t r0 = tx;
   uint32_t r1 = ty;
   return ((Spec_SPARKLE2_branch1){ .fst = r0, .snd = r1 });
 }
 
-Spec_SPARKLE2_branch1 Hacl_Impl_Sparkle_m(uint32_t n, uint32_t *b)
+void
+Hacl_Impl_Sparkle_xor_x(uint32_t n, uint32_t *b, uint32_t lty, uint32_t ltx, uint32_t *temp)
 {
-  Spec_SPARKLE2_branch1 scrut = Hacl_Impl_Sparkle_xor(n, b);
-  uint32_t ltx = scrut.fst;
-  uint32_t lty = scrut.snd;
-  return
-    (
-      (Spec_SPARKLE2_branch1){
-        .fst = (ltx << (uint32_t)16U | ltx >> (uint32_t)16U) ^ (ltx & (uint32_t)0xffffU),
-        .snd = (lty << (uint32_t)16U | lty >> (uint32_t)16U) ^ (lty & (uint32_t)0xffffU)
-      }
-    );
+  for (uint32_t i = (uint32_t)0U; i < n; i++)
+  {
+    uint32_t xi = b[(uint32_t)2U * i];
+    uint32_t yi = b[(uint32_t)2U * i + (uint32_t)1U];
+    uint32_t xi_n = xi ^ lty;
+    uint32_t yi_n = yi ^ ltx;
+    temp[(uint32_t)2U * i] = xi_n;
+    temp[(uint32_t)2U * i + (uint32_t)1U] = yi_n;
+  }
 }
 
-void Hacl_Impl_Sparkle_l_step(uint32_t n, uint32_t *perm, uint32_t i, uint32_t *result)
+void Hacl_Impl_Sparkle_m(uint32_t n, uint32_t *b, uint32_t *temp)
 {
-  uint32_t xi = result[(uint32_t)2U * i];
-  uint32_t yi = result[(uint32_t)2U * i + (uint32_t)1U];
-  uint32_t p0i = perm[(uint32_t)2U * i];
-  uint32_t p1i = perm[(uint32_t)2U * i + (uint32_t)1U];
-  Spec_SPARKLE2_branch1 branchIUpd = { .fst = xi ^ p0i, .snd = yi ^ p1i };
+  uint32_t tx = (uint32_t)0U;
+  uint32_t ty = (uint32_t)0U;
+  for (uint32_t i = (uint32_t)0U; i < n; i++)
+  {
+    uint32_t xi = b[(uint32_t)2U * i];
+    uint32_t yi = b[(uint32_t)2U * i + (uint32_t)1U];
+    uint32_t tx_0 = tx;
+    uint32_t ty_0 = ty;
+    tx = xi ^ tx_0;
+    ty = yi ^ ty_0;
+  }
+  uint32_t r0 = tx;
+  uint32_t r1 = ty;
+  Spec_SPARKLE2_branch1 scrut = { .fst = r0, .snd = r1 };
+  uint32_t ltx = scrut.fst;
+  uint32_t lty = scrut.snd;
+  Hacl_Impl_Sparkle_xor_x(n,
+    b,
+    (lty << (uint32_t)16U | lty >> (uint32_t)16U) ^ (lty & (uint32_t)0xffffU),
+    (ltx << (uint32_t)16U | ltx >> (uint32_t)16U) ^ (ltx & (uint32_t)0xffffU),
+    temp);
+}
+
+void Hacl_Impl_Sparkle_l_step(uint32_t n, uint32_t *right, uint32_t i, uint32_t *m1)
+{
+  uint32_t xi = right[(uint32_t)2U * i];
+  uint32_t yi = right[(uint32_t)2U * i + (uint32_t)1U];
+  uint32_t p0i = m1[(uint32_t)2U * i];
+  uint32_t p1i = m1[(uint32_t)2U * i + (uint32_t)1U];
+  Spec_SPARKLE2_branch1 branchIUpd = { .fst = p0i ^ xi, .snd = p1i ^ yi };
   uint32_t x = branchIUpd.fst;
   uint32_t y = branchIUpd.snd;
-  perm[(uint32_t)2U * i] = x;
-  perm[(uint32_t)2U * i + (uint32_t)1U] = y;
+  m1[(uint32_t)2U * i] = x;
+  m1[(uint32_t)2U * i + (uint32_t)1U] = y;
+}
+
+void Hacl_Impl_Sparkle_l(uint32_t n, uint32_t *b)
+{
+  KRML_CHECK_SIZE(sizeof (uint32_t), n);
+  uint32_t temp[n];
+  memset(temp, 0U, n * sizeof (uint32_t));
+  uint32_t *left = b;
+  uint32_t *right = b + n;
+  Hacl_Impl_Sparkle_m(n >> (uint32_t)1U, left, temp);
+  for (uint32_t i = (uint32_t)0U; i < n >> (uint32_t)1U; i++)
+  {
+    uint32_t xi = right[(uint32_t)2U * i];
+    uint32_t yi = right[(uint32_t)2U * i + (uint32_t)1U];
+    uint32_t p0i = temp[(uint32_t)2U * i];
+    uint32_t p1i = temp[(uint32_t)2U * i + (uint32_t)1U];
+    Spec_SPARKLE2_branch1 branchIUpd = { .fst = p0i ^ xi, .snd = p1i ^ yi };
+    uint32_t x = branchIUpd.fst;
+    uint32_t y = branchIUpd.snd;
+    temp[(uint32_t)2U * i] = x;
+    temp[(uint32_t)2U * i + (uint32_t)1U] = y;
+  }
+  for (uint32_t i = (uint32_t)0U; i < n >> (uint32_t)1U; i++)
+  {
+    Spec_SPARKLE2_branch1
+    left_i = { .fst = left[(uint32_t)2U * i], .snd = left[(uint32_t)2U * i + (uint32_t)1U] };
+    uint32_t x = left_i.fst;
+    uint32_t y = left_i.snd;
+    right[(uint32_t)2U * i] = x;
+    right[(uint32_t)2U * i + (uint32_t)1U] = y;
+  }
+  for (uint32_t i = (uint32_t)0U; i < n >> (uint32_t)1U; i++)
+  {
+    uint32_t index = i - (uint32_t)1U;
+    uint32_t k = n >> (uint32_t)1U;
+    uint32_t j = index % k;
+    Spec_SPARKLE2_branch1
+    temp_i = { .fst = temp[(uint32_t)2U * i], .snd = temp[(uint32_t)2U * i + (uint32_t)1U] };
+    uint32_t x = temp_i.fst;
+    uint32_t y = temp_i.snd;
+    left[(uint32_t)2U * j] = x;
+    left[(uint32_t)2U * j + (uint32_t)1U] = y;
+  }
+}
+
+void Hacl_Impl_Sparkle_add2(uint32_t n, uint32_t i, uint32_t *b)
+{
+  uint32_t x0 = b[0U];
+  uint32_t y0 = b[1U];
+  uint32_t x1 = b[2U];
+  uint32_t y1 = b[3U];
+  uint32_t i0 = i & (uint32_t)7U;
+  uint32_t y01 = y0 ^ Hacl_Impl_Sparkle_rcon[i0];
+  uint32_t y11 = y1 ^ i;
+  b[0U] = x0;
+  b[1U] = y01;
+  b[2U] = x1;
+  b[3U] = y11;
+}
+
+void Hacl_Impl_Sparkle_toBranch(uint32_t n, uint8_t *i, uint32_t *o)
+{
+  for (uint32_t i0 = (uint32_t)0U; i0 < (uint32_t)2U * n; i0++)
+  {
+    uint32_t *os = o;
+    uint8_t *bj = i + i0 * (uint32_t)4U;
+    uint32_t u = load32_le(bj);
+    uint32_t r = u;
+    uint32_t x = r;
+    os[i0] = x;
+  }
+}
+
+void Hacl_Impl_Sparkle_fromBranch(uint32_t n, uint32_t *i, uint8_t *o)
+{
+  for (uint32_t i0 = (uint32_t)0U; i0 < (uint32_t)2U * n; i0++)
+  {
+    store32_le(o + i0 * (uint32_t)4U, i[i0]);
+  }
 }
 
 void Hacl_Impl_Sparkle_arx_n_step(uint32_t n, uint32_t i, uint32_t *b)
@@ -113,112 +209,60 @@ void Hacl_Impl_Sparkle_arx_n_step(uint32_t n, uint32_t i, uint32_t *b)
   b[(uint32_t)2U * i + (uint32_t)1U] = y;
 }
 
-typedef struct __Spec_SPARKLE2_branch1_Spec_SPARKLE2_branch1_Spec_SPARKLE2_branch1_s
-{
-  Spec_SPARKLE2_branch1 fst;
-  Spec_SPARKLE2_branch1 snd;
-  Spec_SPARKLE2_branch1 thd;
-}
-__Spec_SPARKLE2_branch1_Spec_SPARKLE2_branch1_Spec_SPARKLE2_branch1;
-
 void Hacl_Impl_Sparkle_sparkle256(uint32_t steps, uint8_t *i, uint8_t *o)
 {
-  uint32_t temp[12U] = { 0U };
-  for (uint32_t i0 = (uint32_t)0U; i0 < (uint32_t)8U; i0++)
+  uint32_t len = (uint32_t)4U;
+  KRML_CHECK_SIZE(sizeof (uint32_t), len * (uint32_t)2U);
+  uint32_t temp[len * (uint32_t)2U];
+  memset(temp, 0U, len * (uint32_t)2U * sizeof (uint32_t));
+  Hacl_Impl_Sparkle_toBranch(len, i, temp);
+  for (uint32_t i0 = (uint32_t)0U; i0 < steps; i0++)
   {
-    uint32_t *os = temp;
-    uint8_t *bj = i + i0 * (uint32_t)4U;
-    uint32_t u = load32_le(bj);
-    uint32_t r = u;
-    uint32_t x = r;
-    os[i0] = x;
+    Hacl_Impl_Sparkle_add2(len, i0, temp);
+    for (uint32_t i1 = (uint32_t)0U; i1 < len; i1++)
+    {
+      Hacl_Impl_Sparkle_arx_n_step(len, i1, temp);
+    }
+    Hacl_Impl_Sparkle_l(len, temp);
   }
-  for (uint32_t i1 = (uint32_t)0U; i1 < steps; i1++)
+  Hacl_Impl_Sparkle_fromBranch(len, temp, o);
+}
+
+void Hacl_Impl_Sparkle_sparkle384(uint32_t steps, uint8_t *i, uint8_t *o)
+{
+  uint32_t len = (uint32_t)6U;
+  KRML_CHECK_SIZE(sizeof (uint32_t), len * (uint32_t)2U);
+  uint32_t temp[len * (uint32_t)2U];
+  memset(temp, 0U, len * (uint32_t)2U * sizeof (uint32_t));
+  Hacl_Impl_Sparkle_toBranch(len, i, temp);
+  for (uint32_t i0 = (uint32_t)0U; i0 < steps; i0++)
   {
-    uint32_t x00 = temp[0U];
-    uint32_t y00 = temp[1U];
-    uint32_t x1 = temp[2U];
-    uint32_t y1 = temp[3U];
-    uint32_t i0 = i1 & (uint32_t)7U;
-    uint32_t y010 = y00 ^ Hacl_Impl_Sparkle_rcon[i0];
-    uint32_t y11 = y1 ^ i1;
-    temp[0U] = x00;
-    temp[1U] = y010;
-    temp[2U] = x1;
-    temp[3U] = y11;
+    Hacl_Impl_Sparkle_add2(len, i0, temp);
+    for (uint32_t i1 = (uint32_t)0U; i1 < len; i1++)
     {
-      Hacl_Impl_Sparkle_arx_n_step((uint32_t)4U, (uint32_t)0U, temp);
+      Hacl_Impl_Sparkle_arx_n_step(len, i1, temp);
     }
-    {
-      Hacl_Impl_Sparkle_arx_n_step((uint32_t)4U, (uint32_t)1U, temp);
-    }
-    {
-      Hacl_Impl_Sparkle_arx_n_step((uint32_t)4U, (uint32_t)2U, temp);
-    }
-    {
-      Hacl_Impl_Sparkle_arx_n_step((uint32_t)4U, (uint32_t)3U, temp);
-    }
-    Spec_SPARKLE2_branch1 scrut = Hacl_Impl_Sparkle_m((uint32_t)4U, temp);
-    uint32_t ltx = scrut.fst;
-    uint32_t lty = scrut.snd;
-    uint32_t x0 = (uint32_t)0U;
-    uint32_t y0 = (uint32_t)0U;
-    x0 = temp[0U];
-    y0 = temp[1U];
-    {
-      Spec_SPARKLE2_branch1
-      branch_j_nb =
-        {
-          .fst = temp[(uint32_t)2U * ((uint32_t)0U + (uint32_t)1U + (uint32_t)2U)],
-          .snd = temp[(uint32_t)2U * ((uint32_t)0U + (uint32_t)1U + (uint32_t)2U) + (uint32_t)1U]
-        };
-      Spec_SPARKLE2_branch1
-      branch_j =
-        {
-          .fst = temp[(uint32_t)2U * ((uint32_t)0U + (uint32_t)1U)],
-          .snd = temp[(uint32_t)2U * ((uint32_t)0U + (uint32_t)1U) + (uint32_t)1U]
-        };
-      __Spec_SPARKLE2_branch1_Spec_SPARKLE2_branch1_Spec_SPARKLE2_branch1
-      scrut0 = { .fst = branch_j_nb, .snd = branch_j, .thd = { .fst = lty, .snd = ltx } };
-      uint32_t i2y = scrut0.thd.snd;
-      uint32_t i2x = scrut0.thd.fst;
-      uint32_t i1y = scrut0.snd.snd;
-      uint32_t i1x = scrut0.snd.fst;
-      uint32_t i0y = scrut0.fst.snd;
-      uint32_t i0x = scrut0.fst.fst;
-      uint32_t o0_x = i0x ^ (i1x ^ i2x);
-      uint32_t o0_y = i0y ^ (i1y ^ i2y);
-      Spec_SPARKLE2_branch1 b0 = { .fst = o0_x, .snd = o0_y };
-      uint32_t x = b0.fst;
-      uint32_t y2 = b0.snd;
-      temp[(uint32_t)2U * (uint32_t)0U] = x;
-      temp[(uint32_t)2U * (uint32_t)0U + (uint32_t)1U] = y2;
-      uint32_t x2 = temp[(uint32_t)2U * ((uint32_t)0U + (uint32_t)1U)];
-      uint32_t y = temp[(uint32_t)2U * ((uint32_t)0U + (uint32_t)1U) + (uint32_t)1U];
-      temp[(uint32_t)2U * ((uint32_t)0U + (uint32_t)1U + (uint32_t)2U)] = x2;
-      temp[(uint32_t)2U * ((uint32_t)0U + (uint32_t)1U + (uint32_t)2U) + (uint32_t)1U] = y;
-    }
-    uint32_t x01 = x0;
-    uint32_t y01 = y0;
-    uint32_t i0x = temp[4U];
-    uint32_t i0y = temp[5U];
-    uint32_t i1x = x01;
-    uint32_t i1y = y01;
-    uint32_t i2x = lty;
-    uint32_t i2y = ltx;
-    uint32_t o0_x = i0x ^ (i1x ^ i2x);
-    uint32_t o0_y = i0y ^ (i1y ^ i2y);
-    Spec_SPARKLE2_branch1 last0 = { .fst = o0_x, .snd = o0_y };
-    uint32_t x = last0.fst;
-    uint32_t y = last0.snd;
-    temp[(uint32_t)2U * ((uint32_t)2U - (uint32_t)1U)] = x;
-    temp[(uint32_t)2U * ((uint32_t)2U - (uint32_t)1U) + (uint32_t)1U] = y;
-    temp[4U] = x01;
-    temp[5U] = y01;
+    Hacl_Impl_Sparkle_l(len, temp);
   }
-  for (uint32_t i0 = (uint32_t)0U; i0 < (uint32_t)8U; i0++)
+  Hacl_Impl_Sparkle_fromBranch(len, temp, o);
+}
+
+void Hacl_Impl_Sparkle_sparkle512(uint32_t steps, uint8_t *i, uint8_t *o)
+{
+  uint32_t len = (uint32_t)8U;
+  KRML_CHECK_SIZE(sizeof (uint32_t), len * (uint32_t)2U);
+  uint32_t temp[len * (uint32_t)2U];
+  memset(temp, 0U, len * (uint32_t)2U * sizeof (uint32_t));
+  Hacl_Impl_Sparkle_toBranch(len, i, temp);
+  for (uint32_t i0 = (uint32_t)0U; i0 < steps; i0++)
   {
-    store32_le(o + i0 * (uint32_t)4U, temp[i0]);
+    Hacl_Impl_Sparkle_add2(len, i0, temp);
+    for (uint32_t i1 = (uint32_t)0U; i1 < len; i1++)
+    {
+      Hacl_Impl_Sparkle_arx_n_step(len, i1, temp);
+    }
+    Hacl_Impl_Sparkle_l(len, temp);
   }
+  Hacl_Impl_Sparkle_fromBranch(len, temp, o);
 }
 
