code/experimental/SPARKLE/Hacl.Impl.Sparkle.fst
@@ -9,13 +9,10 @@ open Lib.ByteBuffer
 open Lib.Buffer
 
 open Spec.SPARKLE2
-open FStar.Mul
 
 
-#set-options " --z3rlimit 200"
+#set-options " --z3rlimit 200 --ifuel 0 --fuel 0"
 
-inline_for_extraction
-let size_word: size_t = 4ul
 
 inline_for_extraction
 let vsize_rcon: size_t = 8ul
@@ -26,7 +23,8 @@ let rcon: x: glbuffer uint32 vsize_rcon
   createL_global rcon_list
 
 
-type branch_len =  n: size_t {v n = 1 \/ v n = 2 \/ v n = 3 \/ v n = 4 \/ v n = 6 \/ v n = 8}
+type branch_len = n: size_t {v n = 1 \/ v n = 2 \/ v n = 3 \/ v n = 4 \/ v n = 6 \/ v n = 8}
+
 
 inline_for_extraction noextract
 type branch branch_len = lbuffer uint32 (2ul *! branch_len)
@@ -53,10 +51,11 @@ let setBranch #n i (x, y) b =
   upd #uint32 b (2ul *! i) x; upd #uint32 b (2ul *! i +! 1ul) y
 
 
+inline_for_extraction noextract
 val xor_step: #l: branch_len -> b: branch l
   -> tx: lbuffer uint32 (size 1) 
   -> ty: lbuffer uint32 (size 1) 
-  -> i: size_t {v i <= v l / 2} ->
+  -> i: size_t {v i < v l} ->
   Stack unit
   (requires fun h -> live h b /\ live h tx /\ live h ty /\ disjoint tx ty)
   (ensures fun h0 _ h1 -> modifies (loc tx |+| loc ty) h0 h1 /\ (
@@ -74,6 +73,7 @@ let xor_step #l b tx ty i =
   upd ty (size 0) (yi ^. ty_0)
 
 
+inline_for_extraction
 val xor: #l: branch_len -> b: branch l -> Stack (tuple2 uint32 uint32)
     (requires fun h -> live h b)
     (ensures fun h0 r h1 -> modifies0 h0 h1 /\ r == Spec.SPARKLE2.xor #(v l) (as_seq h0 b))
@@ -83,7 +83,7 @@ let xor #l b =
     let tx = create (size 1) (u32 0) in 
     let ty = create (size 1) (u32 0) in 
   let h0 = ST.get() in 
-  let inv h (i: nat {i <= v l / 2})  = live h b /\ live h ty /\ live h tx /\ 
+  let inv h (i: nat {i <= v l})  = live h b /\ live h ty /\ live h tx /\ 
     disjoint tx ty /\ disjoint tx b /\ disjoint ty b /\
     modifies (loc tx |+| loc ty) h0 h /\ (
       let tx_0 = Lib.Sequence.index (as_seq h0 tx) 0 in 
@@ -94,103 +94,154 @@ let xor #l b =
 	Lib.LoopCombinators.repeati #(tuple2 uint32 uint32) i (Spec.SPARKLE2.xor_step #(v l) (as_seq h0 b)) (tx_0, ty_0)) in 
   Lib.LoopCombinators.eq_repeati0 (v l / 2 + 1) (Spec.SPARKLE2.xor_step #(v l) (as_seq h0 b)) (
     Lib.Sequence.index (as_seq h0 tx) 0, Lib.Sequence.index (as_seq h0 ty) 0);
-    
-  Lib.Loops.for 0ul (l >>. 1ul) inv
-    (fun (i: size_t {v i < v l / 2}) -> 
+
+  Lib.Loops.for 0ul l inv
+    (fun (i: size_t {v i < v l}) -> 
       xor_step b tx ty i;
       let f = Spec.SPARKLE2.xor_step #(v l) (as_seq h0 b) in 
       
       let tx_0 = Lib.Sequence.index (as_seq h0 tx) 0 in 
       let ty_0 = Lib.Sequence.index (as_seq h0 ty) 0 in 
-      Lib.LoopCombinators.unfold_repeati (v l / 2 + 1) f (tx_0, ty_0) (v i));
+      Lib.LoopCombinators.unfold_repeati (v l) f (tx_0, ty_0) (v i));
   let r0, r1 = index tx (size 0), index ty (size 0) in 
   pop_frame();
   r0, r1
 
-
-
-val m: #l: branch_len -> b: branch l ->  Stack (tuple2 uint32 uint32)
-  (requires fun h -> live h b)
-  (ensures fun h0 r h1 -> modifies (loc b) h0 h1)
-
-let m #n b = 
-  let ltx, lty = xor #n b in 
-  (l1 ltx, l1 lty)
+open FStar.Mul
 
 
 inline_for_extraction noextract
-val xor_3: i0: tuple2 uint32 uint32  -> i1: tuple2 uint32 uint32  -> i2: tuple2 uint32 uint32 -> 
-  Stack (tuple2 uint32 uint32) 
-    (requires fun h -> true)
-    (ensures fun h0 _ h1 -> modifies0 h0 h1)
+val xor_x_step: #n: branch_len -> b: branch n -> lty: uint32 -> ltx: uint32 -> i: size_t {v i < v n}
+  -> temp: branch n ->
+  Stack unit 
+  (requires fun h -> live h b /\ live h temp)
+  (ensures fun h0 _ h1 -> modifies (loc temp) h0 h1 /\ (
+    as_seq h1 temp == xor_x_step #(v n) (lty, ltx) (as_seq h0 b) (v i) (as_seq h0 temp)))
 
-let xor_3 (i0x, i0y) (i1x, i1y) (i2x, i2y)  = 
-  let o0_x = i0x ^. i1x ^. i2x in 
-  let o0_y = i0y ^. i1y ^. i2y in   
-  o0_x, o0_y
+let xor_x_step #n b lty ltx i temp = 
+  let xi, yi = getBranch b i in
+  let xi_n = xi ^. lty in
+  let yi_n = yi ^. ltx in
+  setBranch i (xi_n, yi_n) temp
 
+
+val xor_x: #n: branch_len -> b: branch n -> lty: uint32 -> ltx: uint32 -> temp: branch n -> Stack unit 
+  (requires fun h -> live h b /\ live h temp /\ disjoint temp b)
+  (ensures fun h0 _ h1 -> modifies (loc temp) h0 h1 /\ (
+    as_seq h1 temp == xor_x #(v n) (as_seq h0 b) (lty, ltx) (as_seq h0 temp)))
+
+let xor_x #n b lty ltx temp = 
+  let h0 = ST.get() in 
+  Lib.LoopCombinators.eq_repeati0 (v n) (
+    (Spec.SPARKLE2.xor_x_step #(v n) (lty, ltx) (as_seq h0 b))) (as_seq h0 temp);
+ 
+  let inv h (i: nat {i >= 0 /\ i <= v n})  = live h b /\ modifies (loc temp) h0 h /\ (
+    let f = Spec.SPARKLE2.xor_x_step #(v n) (lty, ltx) (as_seq h0 b) in 
+    let temp0 = as_seq h0 temp in
+    as_seq h temp == Lib.LoopCombinators.repeati i f temp0) in   
+
+  Lib.Loops.for 0ul n inv (fun (i: size_t {v i < v n}) -> 
+    xor_x_step b lty ltx i temp;
+    let f = Spec.SPARKLE2.xor_x_step #(v n) (lty, ltx) (as_seq h0 b) in
+    let temp0 = as_seq h0 temp in
+    Lib.LoopCombinators.unfold_repeati (v n) f temp0 (v i)
+  )
+
+
+val m: #n: branch_len -> b: branch n -> temp: branch n -> Stack unit 
+  (requires fun h -> live h b /\ live h temp /\ disjoint temp b)
+  (ensures fun h0 _ h1 -> modifies (loc temp) h0 h1 /\ as_seq h1 temp == Spec.SPARKLE2.m #(v n) (as_seq h0 b) (as_seq h0 temp))
+
+let m #n b temp  = 
+  let ltx, lty = xor #n b  in 
+  xor_x #n b (l1 lty) (l1 ltx) temp
 
 
 inline_for_extraction
-val l_step: #n: branch_len -> perm: branch n -> i: size_t {2 * v i <= v n} 
-  -> rightBranch: branch n -> Stack unit 
-  (requires fun h -> live h perm /\ live h rightBranch)
-  (ensures fun h0 _ h1 -> modifies (loc perm) h0 h1)
+val l_step: #n: branch_len -> right: branch n -> i: size_t {v i < v n} -> m: branch n -> Stack unit 
+  (requires fun h -> live h m /\ live h right)
+  (ensures fun h0 _ h1 -> modifies (loc m) h0 h1 /\ 
+    as_seq h1 m == Spec.SPARKLE2.l0_step #(v n) (as_seq h0 right) (v i) (as_seq h0 m))
 
-let l_step #n perm i result = 
-  let xi, yi = getBranch result i in 
-  let p0i, p1i = getBranch perm i in
-  let branchIUpd = xi ^. p0i, yi ^. p1i in
-  setBranch #n i branchIUpd perm
+let l_step #n right i m = 
+  let xi, yi = getBranch right i in 
+  let p0i, p1i = getBranch m i in 
+  let branchIUpd = p0i ^. xi, p1i ^. yi in
+  setBranch i branchIUpd m
 
-inline_for_extraction noextract
+
 val l: #n: branch_len {v n % 2 == 0} -> b: branch n -> Stack unit 
   (requires fun h -> live h b)
-  (ensures fun h0 _ h1 -> modifies (loc b) h0 h1)
-
+  (ensures fun h0 _ h1 -> modifies (loc b) h0 h1 /\ as_seq h1 b ==  Spec.SPARKLE2.l #(v n) (as_seq h0 b))
 
 let l #n b = 
-  let h0 = ST.get() in 
-  let leftBranch = sub b (size 0) n in 
-  let rightBranch = sub b n n in 
-
-  let ltx, lty = m #n b in 
-
   push_frame(); 
-  let x0 = create (size 1) (u32 0) in 
-  let y0 = create (size 1) (u32 0) in
-
-  upd x0 (size 0) (index b (size 0)); 
-  upd y0 (size 0) (index b (size 1));
-
-  Lib.Loops.for 0ul ((n -! 2ul) >>. 1ul)
-    (fun h i -> live h b /\ modifies (loc b) h0 h)
-    (fun (i: size_t) ->
-      assert(v i < v ( n  >>. 2ul)) ;
-      admit(); 
-      assume (v (i +. 1ul +. (n >>. 1ul)) < v n);
-      let branch_j_nb = getBranch #n b (i +. 1ul +. (n >>. 1ul)) in 
-	admit(); 
-      let branch_j = getBranch #n b (i +. 1ul) in 
-      let b0 = xor_3 branch_j_nb branch_j (lty, ltx) in
-      setBranch #n i b0 b;
-      setBranch #n (i +. 1ul +. (n >>. 1ul)) (getBranch #n b (i +. 1ul)) b);
-  admit();
+    let temp : branch (n >>. 1ul) = create n (u32 0) in 
+    let left : branch (n >>. 1ul) = sub b (size 0) n in 
+    let right : branch (n >>. 1ul) = sub b n n in
+    let h = ST.get() in 
   
-    let x0 = index x0 (size 0) in 
-    let y0 = index y0 (size 0) in 
-    let last0 = xor_3 (getBranch #n b (n >>. 1ul)) (x0, y0) (lty, ltx) in 
-    setBranch #n ((n >>. 1ul) -. 1ul) last0 b;
-    setBranch #n (n >>. 1ul) (x0, y0) b;
+  m left temp;
+  
+
+  let h0 = ST.get() in
+  let inv0 h (i: nat {i <= v n / 2}) = 
+    let f0 = Spec.SPARKLE2.l0_step #(v n / 2) (as_seq h0 right) in 
+    modifies (loc temp) h0 h /\ disjoint temp right /\
+    as_seq h temp == Lib.LoopCombinators.repeati #(Spec.SPARKLE2.branch (v n / 2)) i f0 (as_seq h0 temp) in 
+
+  Lib.LoopCombinators.eq_repeati0 (v n / 2) (Spec.SPARKLE2.l0_step #(v n / 2) (as_seq h0 right)) (as_seq h0 temp);
+  Lib.Loops.for 0ul (n >>. 1ul) inv0 
+    (fun (i: size_t {v i < v n / 2}) -> 
+      l_step right i temp;
+      let f = Spec.SPARKLE2.l0_step #(v n / 2) (as_seq h0 right) in 
+      Lib.LoopCombinators.unfold_repeati (v n / 2) f (as_seq h0 temp) (v i)); 
+    
+  let h1 = ST.get() in 
+  Lib.LoopCombinators.eq_repeati0 (v n / 2) (l1_step #(v n / 2) (as_seq h1 left)) (as_seq h1 right);
+
+  Lib.Loops.for 0ul (n >>. 1ul)
+    (fun h i -> modifies (loc right) h1 h /\ disjoint left right /\ (
+      let f1 = l1_step #(v n / 2) (as_seq h1 left) in 
+      as_seq h right == Lib.LoopCombinators.repeati #(Spec.SPARKLE2.branch (v n / 2)) i f1 (as_seq h1 right)))
+
+    (fun (i: size_t {v i < v n / 2}) -> 
+      let h0_ = ST.get() in 
+
+      let left_i = getBranch left i in 
+      setBranch i left_i right;
+      
+      let f = l1_step #(v n / 2) (as_seq h1 left) in 
+      Lib.LoopCombinators.unfold_repeati (v n / 2) f (as_seq h1 right) (v i));
+      
+
+  let h2 = ST.get() in 
+  Lib.LoopCombinators.eq_repeati0 (v n / 2) (l2_step #(v n / 2) (as_seq h1 temp)) (as_seq h2 left);
+  Lib.Loops.for 0ul (n >>. 1ul)
+    (fun h i -> modifies (loc left) h2 h /\ disjoint left temp /\  (
+      let f2 = l2_step #(v n / 2) (as_seq h1 temp) in 
+      as_seq h left == Lib.LoopCombinators.repeati #(Spec.SPARKLE2.branch (v n / 2)) i f2 (as_seq h2 left)))
+    (fun (i: size_t {v i < v n / 2}) -> 
+      let index = Lib.RawIntTypes.size_to_UInt32 (i -. 1ul) in 
+      let k =  Lib.RawIntTypes.size_to_UInt32 (n >>. 1ul) in 
+      let j = FStar.UInt32.rem index k in 
+
+      let temp_i = getBranch temp i in 
+      setBranch j temp_i left;
+
+      let f2 = l2_step #(v n / 2) (as_seq h1 temp) in 
+      Lib.LoopCombinators.unfold_repeati (v n / 2) f2 (as_seq h2 left) (v i));
+
+  let h3 = ST.get() in
+  Lib.Sequence.lemma_concat2 (v n) (as_seq h3 left) (v n) (as_seq h3 right) (as_seq h3 b);
   pop_frame()
 
-inline_for_extraction noextract
-val add2: #n: branch_len {v n >= 4} -> i: size_t -> b:branch n -> Stack unit 
+
+val add2: #n: branch_len {v n > 1} -> i: size_t -> b:branch n -> Stack unit 
   (requires fun h -> live h b) 
-  (ensures fun h0 _ h1 -> modifies (loc b) h0 h1)
+  (ensures fun h0 _ h1 -> modifies (loc b) h0 h1 /\ as_seq h1 b == Spec.SPARKLE2.add2 #(v n) (v i) (as_seq h0 b))
 
 let add2 #n i b = 
-
   recall_contents rcon (Lib.Sequence.of_list rcon_list); 
 
   let (x0, y0) = getBranch #n b (size 0) in 
@@ -204,29 +255,29 @@ let add2 #n i b =
   setBranch (size 0) (x0, y0) b;
   setBranch #n (size 1) (x1, y1) b
 
-inline_for_extraction noextract
+
 val toBranch: #n: branch_len -> i: lbuffer uint8 (size 8 *! n) -> o: branch n -> 
   Stack unit 
   (requires fun h -> live h i /\ live h o /\ disjoint i o)
-  (ensures fun h0 _ h1 -> True)
+  (ensures fun h0 _ h1 -> modifies (loc o) h0 h1 /\ as_seq h1 o == Spec.SPARKLE2.toBranch #(v n) (as_seq h0 i))
 
 let toBranch #n i o = 
   uints_from_bytes_le o i 
 
-inline_for_extraction noextract
+
 val fromBranch: #n: branch_len -> i: branch n -> o: lbuffer uint8 (size 8 *! n) -> 
   Stack unit 
   (requires fun h -> live h i /\ live h o /\ disjoint i o)
-  (ensures fun h0 _ h1 -> True)
+  (ensures fun h0 _ h1 -> modifies (loc o) h0 h1 /\ as_seq h1 o == Spec.SPARKLE2.fromBranch #(v n) (as_seq h0 i))
 
 let fromBranch #n i o = 
   uints_to_bytes_le (2ul *! n) o i
 
 
-val arx_n_step: #n: branch_len -> i: size_t {v i < v n / 2} -> b: branch n -> 
+val arx_n_step: #n: branch_len -> i: size_t {v i < v n} -> b: branch n -> 
   Stack unit 
   (requires fun h -> live h b)
-  (ensures fun h0 _ h1 -> True)
+  (ensures fun h0 _ h1 -> modifies (loc b) h0 h1 /\ as_seq h1 b == Spec.SPARKLE2.arx_n_step #(v n) (v i) (as_seq h0 b))
 
 let arx_n_step #n i b = 
   let branchI = getBranch b i in  
@@ -234,51 +285,93 @@ let arx_n_step #n i b =
   let rcon_i = index rcon i in 
   let x, y = arx rcon_i branchI in 
   setBranch i (x, y) b
+  
 
 inline_for_extraction noextract
-val arx_n: #n: branch_len -> branch n -> 
+val arx_n: #n: branch_len -> b: branch n -> 
   Stack unit 
-  (requires fun h -> True)
-  (ensures fun h0 _ h1 -> True)
+  (requires fun h -> live h b)
+  (ensures fun h0 _ h1 -> modifies (loc b) h0 h1 /\ as_seq h1 b == Spec.SPARKLE2.arx_n #(v n) (as_seq h0 b)) 
 
 let arx_n #n b =
-  Lib.Loops.for 0ul n
-  (fun h i -> live h b)
-  (fun (i: size_t {v i < v n / 2}) -> arx_n_step i b)
+  let h0 = ST.get() in 
+  Lib.LoopCombinators.eq_repeati0 (v n) (Spec.SPARKLE2.arx_n_step #(v n)) (as_seq h0 b);
+
+  Lib.Loops.for 0ul n 
+    (fun h i -> live h b /\ modifies (loc b) h0 h /\ as_seq h b == Lib.LoopCombinators.repeati i (Spec.SPARKLE2.arx_n_step #(v n)) (as_seq h0 b))
+    (fun (i: size_t {v i < v n}) -> arx_n_step i b;
+      Lib.LoopCombinators.unfold_repeati (v n) (Spec.SPARKLE2.arx_n_step #(v n)) (as_seq h0 b) (v i))
+
 
 inline_for_extraction noextract
-val mainLoop_step: #n: branch_len {v n >= 4 /\ v n % 2 == 0 } ->  i: size_t -> branch n ->
+val mainLoop_step: #n: branch_len {v n % 2 == 0} -> i: size_t -> b: branch n ->
   Stack unit 
-  (requires fun h -> True)
-  (ensures fun h0 _ h1 -> True)
-
+  (requires fun h -> live h b)
+  (ensures fun h0 _ h1 -> modifies (loc b) h0 h1 /\ as_seq h1 b == Spec.SPARKLE2.mainLoop_step #(v n) (v i) (as_seq h0 b))
 
 let mainLoop_step #n i b = 
-  add2 i b;
+  add2 #n i b;
   arx_n #n b;
   l #n b
 
+
 inline_for_extraction noextract
-val mainLoop: #n: branch_len {v n >= 4 /\ v n % 2 == 0} -> b: branch n -> steps: size_t -> 
+val mainLoop: #n: branch_len {v n % 2 == 0} -> b: branch n -> steps: size_t -> 
   Stack unit 
-  (requires fun h -> True)
-  (ensures fun h0 _ h1 -> True)
+  (requires fun h -> live h b)
+  (ensures fun h0 _ h1 -> modifies (loc b) h0 h1 /\ as_seq h1 b == Spec.SPARKLE2.mainLoop #(v n) (as_seq h0 b) (v steps))
 
 let mainLoop #n b steps = 
+  let h0 = ST.get() in 
+  Lib.LoopCombinators.eq_repeati0 (v steps) (Spec.SPARKLE2.mainLoop_step #(v n)) (as_seq h0 b);
   Lib.Loops.for 0ul steps
-  (fun h i -> live h b)
-  (fun (i: size_t) -> mainLoop_step i b)
+    (fun h i -> live h b /\ modifies (loc b) h0 h /\ as_seq h b == Spec.SPARKLE2.mainLoop #(v n) (as_seq h0 b) i)
+    (fun i -> 
+      mainLoop_step i b; 
+      let f = Spec.SPARKLE2.mainLoop_step #(v n) in 
+      Lib.LoopCombinators.unfold_repeati (v steps) f (as_seq h0 b) (v i))
 
 
 val sparkle256: steps: size_t -> i: lbuffer (uint8) (size 32) -> o: lbuffer (uint8) (size 32) ->
   Stack unit 
   (requires fun h -> live h i /\ live h o)
-  (ensures fun h0 _ h1 -> True)
+  (ensures fun h0 _ h1 -> modifies (loc o) h0 h1 /\ as_seq h1 o == Spec.SPARKLE2.sparkle256 (v steps) (as_seq h0 i))
 
 let sparkle256 steps i o =
   push_frame();
-    let temp = create (size 12) (u32 0) in 
-    toBranch #(size 4) i temp;
-    mainLoop #(size 4) temp steps;
-    fromBranch #(size 4) temp o; 
+    let len = size 4 in 
+    let temp = create (len *. 2ul) (u32 0) in 
+    toBranch #len i temp;
+    mainLoop #len temp steps;
+    fromBranch #len temp o; 
+  pop_frame()
+
+
+val sparkle384: steps: size_t -> i: lbuffer (uint8) (size 48) -> o: lbuffer (uint8) (size 48) ->
+  Stack unit 
+  (requires fun h -> live h i /\ live h o)
+  (ensures fun h0 _ h1 -> modifies (loc o) h0 h1 /\ as_seq h1 o == Spec.SPARKLE2.sparkle384 (v steps) (as_seq h0 i))
+
+let sparkle384 steps i o =
+  push_frame();
+    let len = size 6 in 
+    let temp = create (len *. 2ul) (u32 0) in 
+    toBranch #len i temp;
+    mainLoop #len temp steps;
+    fromBranch #len temp o; 
+  pop_frame()
+
+
+val sparkle512: steps: size_t -> i: lbuffer (uint8) (size 64) -> o: lbuffer (uint8) (size 64) ->
+  Stack unit 
+  (requires fun h -> live h i /\ live h o)
+  (ensures fun h0 _ h1 -> modifies (loc o) h0 h1 /\ as_seq h1 o == Spec.SPARKLE2.sparkle512 (v steps) (as_seq h0 i))
+
+let sparkle512 steps i o =
+  push_frame();
+    let len = size 8 in 
+    let temp = create (len *. 2ul) (u32 0) in 
+    toBranch #len i temp;
+    mainLoop #len temp steps;
+    fromBranch #len temp o; 
   pop_frame()
